Start working on proof of aux size constant

LeanSorting/Basic.lean
@@ -14,25 +14,24 @@ theorem idk2 {p a : Prop} {h : p} (h_imp : p → a) : a :=
 theorem idk3 {k₁ k₂ start₂ end₂ : ℕ} {h : ¬(k₁ < start₂ ∧ k₂ < end₂)}
     : (¬(k₁ < start₂)) ∨ (¬(k₂ < end₂)) := by
   omega
-
+set_option diagnostics true
 /--
 Merges two ordered contiguous portions of `arr` into `aux`, returning `aux`.
 If there are no other references to `aux`, it will be mutated in-place.
 
 For example,
 ```
-                        region1    region2
+                        chunk1     chunk2
 arr: 1 2 3 100 200 300 [10 20 30 │ 21 22 23] 400 500 600
-aux: 1 2 3 100 200 300 [0  0  0  │ 0  0  0 ] 0   0   0
----> 1 2 3 100 200 300 [10 20 21 │ 22 23 30] 0   0   0
+aux: 1 2 3 100 200 300 [0  0  0  │ 0  0  0 ] 0   0   0    ; before merge
+---> 1 2 3 100 200 300 [10 20 21 │ 22 23 30] 0   0   0    ; after merge
                         │          │         │
 start1 ─────────────────┘          │         │
 start2 ────────────────────────────┘         │
 end2 ────────────────────────────────────────┘
 ```
 -/
-@[inline]
-partial def mergeAdjacentChunksIntoAux [Inhabited α] [Ord α] (arr : Array α) (aux : Array α)
+def mergeAdjacentChunksIntoAux [Ord α] (arr : Array α) (aux : Array α)
     (start₁ : ℕ) (start₂ : ℕ) (end₂ : ℕ)
     (start₁_lt_start₂ : start₁ < start₂)
     (start₂_lt_end₂ : start₂ < end₂)
@@ -105,7 +104,7 @@ partial def mergeAdjacentChunksIntoAux [Inhabited α] [Ord α] (arr : Array α) 
           rw [aux'_def, Array.size_set]
           exact arr_size_eq_aux_size
         have i_succ_def : i.succ = k₁.succ + k₂ - start₂ := by omega
-        let rec loop₁ (aux : Array α) (i : ℕ) (k₁ : ℕ)
+        let rec loop_left (aux : Array α) (i : ℕ) (k₁ : ℕ)
             (arr_size_eq_aux_size : arr.size = aux.size)
             (i_def : i = k₁ + k₂ - start₂)
             : Array α :=
@@ -119,12 +118,13 @@ partial def mergeAdjacentChunksIntoAux [Inhabited α] [Ord α] (arr : Array α) 
               rw [aux'_def, Array.size_set]
               exact arr_size_eq_aux_size
             have i_succ_def : i.succ = k₁.succ + k₂ - start₂ := by omega
-            loop₁ aux' i.succ k₁.succ
+            loop_left aux' i.succ k₁.succ
               arr_size_eq_aux'_size
               i_succ_def
           else
             aux
-        loop₁ aux' i.succ k₁.succ
+        termination_by aux.size - k₁
+        loop_left aux' i.succ k₁.succ
           arr_size_eq_aux'_size
           i_succ_def
       else
@@ -137,7 +137,7 @@ partial def mergeAdjacentChunksIntoAux [Inhabited α] [Ord α] (arr : Array α) 
           rw [aux'_def, Array.size_set]
           exact arr_size_eq_aux_size
         have i_succ_def : i.succ = k₁ + k₂.succ - start₂ := by omega
-        let rec loop₂ (aux : Array α) (i : ℕ) (k₂ : ℕ)
+        let rec loop_right (aux : Array α) (i : ℕ) (k₂ : ℕ)
             (arr_size_eq_aux_size : arr.size = aux.size)
             (i_def : i = k₁ + k₂ - start₂)
             : Array α :=
@@ -150,40 +150,156 @@ partial def mergeAdjacentChunksIntoAux [Inhabited α] [Ord α] (arr : Array α) 
               rw [aux'_def, Array.size_set]
               exact arr_size_eq_aux_size
             have i_succ_def : i.succ = k₁ + k₂.succ - start₂ := by omega
-            loop₂ aux' i.succ k₂.succ
+            loop_right aux' i.succ k₂.succ
               arr_size_eq_aux'_size
               i_succ_def
           else
             aux
-        loop₂ aux' i.succ k₂.succ
+        termination_by aux.size - k₂
+        loop_right aux' i.succ k₂.succ
           arr_size_eq_aux'_size
           i_succ_def
+  termination_by aux.size - i
   loop aux start₁ start₁ start₂
-    (by omega)
-    (by omega)
-    (by omega)
-    (by omega)
-    (by omega)
-    (by omega)
+    arr_size_eq_aux_size
+    (Nat.eq_sub_of_add_eq rfl)
+    (Nat.le_refl start₂)
+    (Nat.lt_succ_of_lt start₁_lt_start₂)
+    (Nat.lt_succ_of_lt start₂_lt_end₂)
+    (fun a ↦ start₂_lt_end₂)
 
-def mergeChunksIntoAux [Inhabited α] [Ord α] (arr : Array α) (aux : Array α)
-    (chunkSize : ℕ) : Array α := Id.run do
+-- theorem mergeAdjacentChunksIntoAux_loop_size_eq
+--     [Ord α]
+--     (arr : Array α) (aux : Array α) (i : ℕ) (k₁ : ℕ) (k₂ : ℕ)
+--     (start₁_lt_stat₂ : i < k₁)
+--     (k₁_lt_k₂ : k₁ < k₂)
+--     (k₂_le_arr_size : k₂ ≤ arr.size)
+--     (arr_size_eq_aux_size : arr.size = aux.size)
+--     (i_def : i = k₁ + k₂ - start₂)
+--     (k₂_ge_start₂ : k₂ ≥ start₂)
+--     (k₁_lt_start₂_succ : k₁ < start₂.succ)
+--     (k₂_lt_end₂_succ : k₂ < end₂.succ)
+--     (k₂_lt_end₂_of_not_k₁_lt_start₂ : ¬k₁ < start₂ → k₂ < end₂)
+--     : (mergeAdjacentChunksIntoAux.loop
+--         arr aux i k₁ k₂
+--         start₁_lt_stat₂
+--         k₁_lt_k₂
+--         k₂_le_arr_size
+--         arr_size_eq_aux_size
+--         ).size = aux.size := by
+--   sorry
+
+#check mergeAdjacentChunksIntoAux.loop.induct 
+
+theorem mergeAdjacentChunksIntoAux_size_eq [Ord α] (arr : Array α) (aux : Array α)
+    (start₁ : ℕ) (start₂ : ℕ) (end₂ : ℕ)
+    (start₁_lt_start₂ : start₁ < start₂)
+    (start₂_lt_end₂ : start₂ < end₂)
+    (end₂_le_arr_size : end₂ ≤ arr.size)
+    (arr_size_eq_aux_size : arr.size = aux.size)
+    : (mergeAdjacentChunksIntoAux arr aux start₁ start₂ end₂
+        start₁_lt_start₂
+        start₂_lt_end₂
+        end₂_le_arr_size
+        arr_size_eq_aux_size).size = aux.size := by
+  unfold mergeAdjacentChunksIntoAux
+  unfold mergeAdjacentChunksIntoAux.loop
+  split
+  next k₁_k₂_in_bounds =>
+    simp []
+    split
+    induction aux, start₁, start₂, end₂,  using mergeAdjacentChunksIntoAux.loop.induct with
+    | case1 => sorry
+    | case2 => sorry
+    | case3 => sorry
+    | case4 => sorry
+    | case5 => sorry
+    -- have ih := (mergeAdjacentChunksIntoAux.loop arr aux start₁ start₂ _ _ _ _ _ _ _ _ _ _ _ _ _ _ _).size = aux.size
+    sorry
+  next k₁_k₁_out_of_bounds =>
+    sorry
+  -- simp? only [mergeAdjacentChunksIntoAux.loop]
+  -- simp [*]
+
+  -- induction (end₂ - start₂) with
+  -- | zero =>
+  --   rw [mergeAdjacentChunksIntoAux.loop]
+  --   simp [*]
+
+  --   split
+  --   . case zero.h_1 =>
+  --     sorry
+  --   . case zero.h_2 =>
+  --     sorry
+  --   . case zero.h_3 =>
+  --     sorry
+  -- | succ n8 =>
+  --   sorry
+  -- -- rw [mergeAdjacentChunksIntoAux.loop]
+  -- -- simp []
+  -- -- split
+  -- -- . case isTrue =>
+  -- --   simp []
+  -- --   split
+  -- --   . case h_1 =>
+  -- --     sorry
+  -- --   . case h_2 =>
+  -- --     sorry
+  -- --   . case h_3 =>
+  -- --     sorry
+  -- -- . case isFalse =>
+  -- --   simp []
+  -- --   rw [mergeAdjacentChunksIntoAux.loop.loop_left]
+  -- --   simp []
+  -- --   split
+  -- --   . case isTrue =>
+  -- --     sorry
+  -- --   . case isFalse =>
+  -- --     rw [Array.size_set]
+
+-- Sorts every two adjacent chunks in `arr` of length `size` into `aux`.
+def mergeChunksIntoAux [Inhabited α] [Ord α] (arr : Array α) (aux : Array α) (size : ℕ)
+    (arr_size_eq_aux_size : arr.size = aux.size)
+    (size_gt_0 : size > 0)
+    : Array α := Id.run do
   let mut aux := aux
-  let mut chunkStart₁ := 0
-  while chunkStart₁ + chunkSize < arr.size do
-    let chunkStart₂ := chunkStart₁ + chunkSize
-    let chunkEnd₂ := min (chunkStart₂ + chunkSize) arr.size
-    aux := mergeAdjacentChunksIntoAux
-                arr aux chunkStart₁ chunkStart₂ chunkEnd₂
-                (by omega) (by omega) (by omega) (by omega)
-    chunkStart₁ := chunkStart₁ + 2 * chunkSize
-  while chunkStart₁ < arr.size do
-    have : chunkStart₁ < arr.size := by omega
-    have chunkStart₁_lt_aux_size : chunkStart₁ < aux.size := by omega
-    aux := aux.set ⟨chunkStart₁, chunkStart₁_lt_aux_size⟩ arr[chunkStart₁]
-    -- aux := (dbgTraceIfShared "mergeChunksIntoAux" aux).set! chunkStart₁ arr[chunkStart₁]!
-    chunkStart₁ := chunkStart₁ + 1
-  pure aux
+  let mut start₁ := 0
+  let rec loop₁ (aux : Array α) (start₁ : ℕ)
+      (arr_size_eq_aux_size : arr.size = aux.size)
+      : Array α :=
+    if start₁ + size < arr.size then
+      let start₂ := start₁ + size
+      let end₂ := min (start₂ + size) arr.size
+      have start₁_lt_start₂ : start₁ < start₂ := by omega
+      have start₂_lt_end₂ : start₂ < end₂ := by omega
+      have end₂_le_arr_size : end₂ ≤ arr.size := by omega
+      let aux' := mergeAdjacentChunksIntoAux
+                   arr aux start₁ start₂ end₂
+                   start₁_lt_start₂
+                   start₂_lt_end₂
+                   end₂_le_arr_size
+                   arr_size_eq_aux_size
+      let start₁' := start₁ + 2 * size
+      have arr_size_eq_aux'_size : arr.size = aux'.size := by
+        apply mergeAdjacentChunksIntoAux_size_eq at aux'
+
+        -- have aux'_def : aux' =
+      loop₁ aux' start₁'
+        arr_size_eq_aux'_size
+    else
+      let rec loop₂ (aux : Array α) (start₁ : ℕ)
+          : Array α :=
+        if start₁ < arr.size then
+          have : start₁ < arr.size := by omega
+          have chunkStart₁_lt_aux_size : start₁ < aux.size := by omega
+          let aux' := aux.set ⟨start₁, chunkStart₁_lt_aux_size⟩ arr[start₁]
+          let start₁' := start₁ + 1
+          loop₂ aux' start₁'
+        else
+          aux
+      loop₂ aux start₁
+  loop₁ aux start₁
+    arr_size_eq_aux_size
 
 @[specialize] def Array.mergeSort [Inhabited α] [Ord α] (arr : Array α) : Array α := Id.run do
   let mut arr := arr
